

Feel free to work with other students, but make sure you write up the homework and code on your own (no copying homework *or* code; no pair programming). Feel free to ask students or instructors for help debugging code or whatever else, though.

1 (Murphy 2.16) Suppose $\theta \sim \text{Beta}(a, b)$ such that

$$\mathbb{P}(\theta; a, b) = \frac{1}{B(a, b)} \theta^{a-1} (1 - \theta)^{b-1} = \frac{\Gamma(a+b)}{\Gamma(a)\Gamma(b)} \theta^{a-1} (1 - \theta)^{b-1}$$

where $B(a, b) = \Gamma(a)\Gamma(b)/\Gamma(a+b)$ is the Beta function and $\Gamma(x)$ is the Gamma function. Derive the mean, mode, and variance of θ .

Start by computing the mean of θ with the given probability distribution $\mathbb{P}(\theta; a, b)$.

$$\mathbb{E}[\theta] = \int_0^1 \theta \mathbb{P}(\theta; a, b) d\theta \quad (1)$$

$$= \int_0^1 \theta \left[\frac{\Gamma(a+b)}{\Gamma(a)\Gamma(b)} \theta^{a-1} (1 - \theta)^{b-1} \right] d\theta \quad (2)$$

$$(3)$$

Recall that

$$\beta(a, b) = \int_0^1 \theta^{a-1} (1 - \theta)^{b-1} d\theta = \frac{\Gamma(a)\Gamma(b)}{\Gamma(a+b)}. \quad (4)$$

Hence, equation (2) becomes

$$\mathbb{E}[\theta] = \frac{\Gamma(a+b)}{\Gamma(a)\Gamma(b)} \int_0^1 \theta^a (1 - \theta)^{b-1} d\theta = \frac{\Gamma(a+b)}{\Gamma(a)\Gamma(b)} \cdot \frac{\Gamma(a+1)\Gamma(b)}{\Gamma(a+1+b)}. \quad (5)$$

Finally, since

$$\Gamma(a+b+1) = (a+b)\Gamma(a+b), \quad (6)$$

equation (5) becomes

$$\mathbb{E}[\theta] = \frac{\Gamma(a+b)}{\Gamma(a)\Gamma(b)} \cdot \frac{\Gamma(a+1)\Gamma(b)}{\Gamma(a+1+b)} = \frac{\Gamma(a+b)}{\Gamma(a)\Gamma(b)} \cdot \frac{a\Gamma(a)\Gamma(b)}{(a+b)\Gamma(a+b)} = \frac{a}{a+b}. \quad (7)$$

Now we compute the mode of θ . This is equivalent to find the solution to the equation

$$\nabla_{\theta} \mathbb{P}(\theta; a, b) = 0. \quad (8)$$

In other words, finding the solution to

$$\nabla_{\theta} \left[\theta^{a-1} (1 - \theta)^{b-1} \right] = 0. \quad (9)$$

This is a simple computation. The left hand side evaluates to

$$(a - 1)\theta^{a-2}(1 - \theta)^{b-1} - (b - 1)\theta^{a-1}(1 - \theta)^{b-2} = 0 \quad (10)$$

which makes equation (9) become

$$(a - 1)\theta^{a-2}(1 - \theta)^{b-1} = (b - 1)\theta^{a-1}(1 - \theta)^{b-2} \quad (11)$$

$$\implies (a + b - 2)\theta = a - 1 \quad (12)$$

$$\implies \theta = \frac{a - 1}{a + b - 2} \quad (13)$$

after cancelling a factor of θ^{a-2} and $(1 - \theta)^{b-2}$ from both sides. This is the mode.

Next we go to the variance! Recall that the variance is defined as

$$\text{Var}[\theta] = \mathbb{E}[\theta^2] - \mathbb{E}[\theta]^2. \quad (14)$$

We automatically have our second term from the first part of this problem. Hence, we focus on computing the first term. But this is simply:

$$\mathbb{E}[\theta^2] = \int_0^1 \theta^2 \mathbb{P}(\theta; a, b) d\theta \quad (15)$$

$$= \int_0^1 \theta^2 \left[\frac{\Gamma(a+b)}{\Gamma(a)\Gamma(b)} \theta^{a-1} (1 - \theta)^{b-1} \right] d\theta \quad (16)$$

$$= \frac{\Gamma(a+b)}{\Gamma(a)\Gamma(b)} \int_0^1 \theta^{a+1} (1 - \theta)^{b-1} d\theta \quad (17)$$

$$= \frac{\Gamma(a+b)}{\Gamma(a)\Gamma(b)} \cdot \frac{\Gamma((a+1)+1)\Gamma(b)}{\Gamma((a+b+1)+1)} \quad (18)$$

$$= \frac{\Gamma(a+b)}{\Gamma(a)\Gamma(b)} \cdot \frac{\Gamma(a)\Gamma(b)}{\Gamma(a+b)} \cdot \frac{(a+1)a}{(a+b+1)(a+b)} \quad (19)$$

$$= \frac{(a+1)a}{(a+b+1)(a+b)}. \quad (20)$$

Therefore,

$$\text{Var}[\theta] = \mathbb{E}[\theta^2] - \mathbb{E}[\theta]^2 \quad (21)$$

$$= \frac{(a+1)a}{(a+b+1)(a+b)} - \frac{a^2}{(a+b)^2} \quad (22)$$

$$= \frac{(a+b)(a+1)a}{(a+b+1)(a+b)^2} - \frac{a^2(a+b+1)}{(a+b)^2(a+b+1)} \quad (23)$$

$$= \frac{(a^2 + a + ba + b)a - a^3 - a^2b - a^2}{(a+b)^2(a+b+1)} \quad (24)$$

$$= \frac{a^3 + a^2 + ba^2 + ba - a^3 - a^2b - a^2}{(a+b)^2(a+b+1)} \quad (25)$$

$$= \frac{ba}{(a+b)^2(a+b+1)}, \quad (26)$$

gives us the variance of θ , as desired.

■

2 (Murphy 9) Show that the multinoulli distribution

$$\text{Cat}(\mathbf{x}|\boldsymbol{\mu}) = \prod_{i=1}^K \mu_i^{x_i}$$

is in the exponential family and show that the generalized linear model corresponding to this distribution is the same as multinoulli logistic regression (softmax regression).

We know that a probability distribution is in the exponential family if it can be expressed as

$$\mathbb{P}(\mathbf{y}; \boldsymbol{\eta}) = b(\mathbf{y}) \exp(\boldsymbol{\eta}^T T(\mathbf{y}) - a(\boldsymbol{\eta})). \quad (27)$$

So, by taking the logarithm and exponentiating both sides (in that order), we have

$$\text{Cat}(\mathbf{x}|\boldsymbol{\mu}) = \exp \left[\log \prod_{i=1}^K \mu_i^{x_i} \right] \quad (28)$$

$$= \exp \left[\sum_{i=1}^K x_i \log \mu_i \right] \quad (29)$$

Here I took a hint from the solutions because I had no idea how to go forward. Apparently, by acknowledging that

$$\sum_{i=1}^K x_i = \sum_{i=1}^{K-1} x_i + x_K = 1 \quad (30)$$

we can make the following substitution from the third to fourth line:

$$\text{Cat}(\mathbf{x}|\boldsymbol{\mu}) = \exp \left[\log \prod_{i=1}^K \mu_i^{x_i} \right] \quad (31)$$

$$= \exp \left[\sum_{i=1}^K x_i \log \mu_i \right] \quad (32)$$

$$= \exp \left[\sum_{i=1}^{K-1} x_i \log \mu_i + x_K \log \mu_K \right] \quad (33)$$

$$= \exp \left[\sum_{i=1}^{K-1} x_i \log \mu_i + \left(1 - \sum_{i=1}^{K-1} x_i \right) \log \mu_K \right] \quad (34)$$

$$= \exp \left[\sum_{i=1}^{K-1} x_i (\log \mu_i - \log \mu_K) + \log \mu_K \right] \quad (35)$$

$$= \exp \left[\sum_{i=1}^{K-1} x_i \log \left(\frac{\mu_i}{\mu_K} \right) + \log \mu_K \right]. \quad (36)$$

Therefore, we can set our canonical parameter to be

$$\boldsymbol{\eta} = \begin{bmatrix} \log\left(\frac{\mu_1}{\mu_K}\right) \\ \vdots \\ \log\left(\frac{\mu_{K-1}}{\mu_K}\right) \end{bmatrix} \quad (37)$$

where we see that $\mu_i = \mu_K e^{\boldsymbol{\eta}_i}$. By substituting this into equation (30),

$$\mu_K = 1 - \mu_K \sum_{i=1}^{K-1} e^{\boldsymbol{\eta}_i} \quad (38)$$

$$\implies \mu_K = \frac{1}{1 + \sum_{i=1}^{K-1} e^{\boldsymbol{\eta}_i}} \quad (39)$$

Hence,

$$\mu_i = \frac{1}{1 + \sum_{i=1}^{K-1} e^{\boldsymbol{\eta}_i}} \cdot e^{\boldsymbol{\eta}_i}. \quad (40)$$

Which finally allows us to write:

$$\text{Cat}(\mathbf{x}|\boldsymbol{\mu}) = \exp(\boldsymbol{\eta}^T \mathbf{x} + \log \mu_K) \quad (41)$$

proving that $\text{Cat}(\mathbf{x}|\boldsymbol{\mu})$ is in the exponential family. Observe that the Softmax function is (Wikipedia)

$$\sigma(\mathbf{z})_i = \frac{e^{z_i}}{\sum_{j=1}^K e^{z_j}} \quad (42)$$

for $i = 1, \dots, K$, which means that the generalized linear model for Cat is the same as the softmax regression. ■